\subsection*{Teil B: Binomische Formeln (30 Minuten)}

    \begin{enumerate}[label=\arabic*.,resume]

    \item \textbf{Erg√§nze die Formeln:}

    \begin{center}
        \begin{tabular}{|c|c|}
            \hline
            1. Binomische Formel & $(a + b)^2 = $ \underline{\hspace{6cm}} \\[2ex]
            \hline
            2. Binomische Formel & $(a - b)^2 = $ \underline{\hspace{6cm}} \\[2ex]  
            \hline
            3. Binomische Formel & $(a + b)(a - b) = $ \underline{\hspace{6cm}} \\[2ex]
            \hline
        \end{tabular}
    \end{center}

    \vspace{1cm}

    \item \textbf{Wende die binomischen Formeln an:}

    \textit{Beispiel:} $(x + 3)^2 = x^2 + 6x + 9$

    \vspace{0.5cm}
    \begin{enumerate}[label=\alph*)]
        \item $(x + 4)^2$ = \underline{\hspace{6cm}}

        \vspace{0.8cm}

        \item $(x - 5)^2$ = \underline{\hspace{6cm}}

        \vspace{0.8cm}

        \item $(2x + 1)^2$ = \underline{\hspace{6cm}}

        \vspace{0.8cm}

        \item $(3x - 2)^2$ = \underline{\hspace{6cm}}

        \vspace{0.8cm}

        \item $(x + 6)(x - 6)$ = \underline{\hspace{6cm}}

        \vspace{0.8cm}

        \item $(2x + 3)(2x - 3)$ = \underline{\hspace{6cm}}

    \end{enumerate}

\end{enumerate}