\subsection*{Teil A: Terme vereinfachen (25 Minuten)}

\begin{enumerate}[label=\arabic*.]

    \item \textbf{Fasse zusammen:}

    \textit{Beispiel:} $3x + 5x = 8x$ \hspace{2cm} $7x - 2x = 5x$

    \vspace{0.5cm}
    \begin{tabular}{ll}
        a) $4x + 7x$ = \underline{\hspace{3cm}} & b) $9x - 3x$ = \underline{\hspace{3cm}} \\[2ex]
        c) $6x^2 + 2x^2$ = \underline{\hspace{3cm}} & d) $8x^2 - 5x^2$ = \underline{\hspace{3cm}} \\[2ex]
        e) $5x + 3y + 2x$ = \underline{\hspace{3cm}} & f) $7a - 2b + 4a$ = \underline{\hspace{3cm}}
    \end{tabular}

    \vspace{1cm}

    \item \textbf{Multipliziere aus:}

    \textit{Beispiel:} $3(x + 4) = 3x + 12$

    \vspace{0.5cm}
    \begin{tabular}{ll}
        a) $5(x + 2)$ = \underline{\hspace{4cm}} & b) $4(3x - 1)$ = \underline{\hspace{4cm}} \\[2ex]
        c) $-2(x + 5)$ = \underline{\hspace{4cm}} & d) $x(x + 3)$ = \underline{\hspace{4cm}} \\[2ex]
        e) $2x(3x - 4)$ = \underline{\hspace{4cm}} & f) $-3x(2x + 1)$ = \underline{\hspace{4cm}}
    \end{tabular}

    \vspace{1cm}

    \item \textbf{Klammere aus:}

    \textit{Beispiel:} $6x + 9 = 3(2x + 3)$

    \vspace{0.5cm}
    \begin{tabular}{ll}
        a) $4x + 8$ = \underline{\hspace{4cm}} & b) $6x - 12$ = \underline{\hspace{4cm}} \\[2ex]
        c) $10x + 15$ = \underline{\hspace{4cm}} & d) $8x^2 + 4x$ = \underline{\hspace{4cm}} \\[2ex]
        e) $12x^2 - 6x$ = \underline{\hspace{4cm}} & f) $15x + 10y$ = \underline{\hspace{4cm}}
    \end{tabular}

\end{enumerate}