\subsection*{Teil B: Binomische Formeln (30 Minuten)}

\begin{enumerate}[label=\arabic*.,resume]

    \item \textbf{Formeln vervollständigen:}

    \begin{center}
        \begin{tabular}{|c|c|}
            \hline
            1. Binomische Formel & $(a + b)^2 = a^2 + $ \underline{\hspace{2cm}} $+ b^2$ \\[2ex]
            \hline
            2. Binomische Formel & $(a - b)^2 = a^2 - $ \underline{\hspace{2cm}} $+ b^2$ \\[2ex]
            \hline
            3. Binomische Formel & $(a + b)(a - b) = a^2 - $ \underline{\hspace{2cm}} \\[2ex]
            \hline
        \end{tabular}
    \end{center}

    \vspace{1cm}

    \item \textbf{Binomische Formeln anwenden:}

    \textit{Beispiel:} $(x + 2)^2 = x^2 + 4x + 4$

    \vspace{0.5cm}
    \begin{enumerate}[label=\alph*)]
        \item $(x + 7)^2$ = \underline{\hspace{6cm}}

        \vspace{0.8cm}

        \item $(x - 4)^2$ = \underline{\hspace{6cm}}

        \vspace{0.8cm}

        \item $(3x + 2)^2$ = \underline{\hspace{6cm}}

        \vspace{0.8cm}

        \item $(2x - 5)^2$ = \underline{\hspace{6cm}}

        \vspace{0.8cm}

        \item $(x + 8)(x - 8)$ = \underline{\hspace{6cm}}

        \vspace{0.8cm}

        \item $(4x + 1)(4x - 1)$ = \underline{\hspace{6cm}}

    \end{enumerate}

    \vspace{1cm}

    \item \textbf{Rückwärts - Faktorisieren:}

    \textit{Beispiel:} $x^2 + 10x + 25 = (x + 5)^2$

    \vspace{0.5cm}
    \begin{tabular}{ll}
        a) $x^2 + 6x + 9$ = \underline{\hspace{4cm}} & b) $x^2 - 8x + 16$ = \underline{\hspace{4cm}} \\[2ex]
        c) $x^2 - 49$ = \underline{\hspace{4cm}} & d) $4x^2 - 16$ = \underline{\hspace{4cm}} \\[2ex]
        e) $9x^2 + 12x + 4$ = \underline{\hspace{4cm}} & f) $25x^2 - 9$ = \underline{\hspace{4cm}}
    \end{tabular}

\end{enumerate}