\subsection*{Teil A: Terme vereinfachen (25 Minuten)}

\begin{enumerate}[label=\arabic*.]

    \item \textbf{Gleichartige Terme zusammenfassen:}

    \textit{Beispiel:} $3x + 5x - 2x = 6x$

    \vspace{0.5cm}
    \begin{tabular}{ll}
        a) $7x + 2x - 3x$ = \underline{\hspace{3cm}} & b) $4x^2 + 3x^2 - x^2$ = \underline{\hspace{3cm}} \\[2ex]
        c) $5a + 3b - 2a + 4b$ = \underline{\hspace{4cm}} & d) $8xy - 3xy + 2xy$ = \underline{\hspace{3cm}} \\[2ex]
        e) $x^2 + 3x + 2x^2 - x$ = \underline{\hspace{4cm}} & f) $6m - 4n + 2m + 7n$ = \underline{\hspace{4cm}}
    \end{tabular}

    \vspace{1cm}

    \item \textbf{Ausmultiplizieren:}

    \textit{Beispiel:} $4(2x - 3) = 8x - 12$

    \vspace{0.5cm}
    \begin{tabular}{ll}
        a) $3(x + 5)$ = \underline{\hspace{4cm}} & b) $-2(3x - 4)$ = \underline{\hspace{4cm}} \\[2ex]
        c) $5(2x + 1)$ = \underline{\hspace{4cm}} & d) $x(x - 6)$ = \underline{\hspace{4cm}} \\[2ex]
        e) $3x(2x + 4)$ = \underline{\hspace{4cm}} & f) $-4x(x - 2)$ = \underline{\hspace{4cm}}
    \end{tabular}

    \vspace{1cm}

    \item \textbf{Ausklammern:}

    \textit{Beispiel:} $6x + 9 = 3(2x + 3)$

    \vspace{0.5cm}
    \begin{tabular}{ll}
        a) $8x + 12$ = \underline{\hspace{4cm}} & b) $15x - 10$ = \underline{\hspace{4cm}} \\[2ex]
        c) $6x^2 + 9x$ = \underline{\hspace{4cm}} & d) $20x^2 - 12x$ = \underline{\hspace{4cm}} \\[2ex]
        e) $14a + 21b$ = \underline{\hspace{4cm}} & f) $18xy - 12x$ = \underline{\hspace{4cm}}
    \end{tabular}

\end{enumerate}