\subsection*{Teil B: Potenzgesetze anwenden (30 Minuten)}

\begin{enumerate}[label=\arabic*.]

    \item \textbf{Potenzen mit gleicher Basis multiplizieren:}
    \textit{Regel:} $a^m \cdot a^n = a^{m+n}$
    \vspace{0.5cm}

    \begin{tabular}{ll}
        a) $2^3 \cdot 2^2$ = $2^{3+2}$ = $2^{\phantom{0}}$ = \underline{\hspace{3cm}} & b) $3^2 \cdot 3^4$ = $3^{\phantom{0}+\phantom{0}}$ = $3^{\phantom{0}}$ = \underline{\hspace{3cm}} \\[3ex]
        c) $5^1 \cdot 5^3$ = $5^{\phantom{0}+\phantom{0}}$ = $5^{\phantom{0}}$ = \underline{\hspace{3cm}} & d) $4^2 \cdot 4^1$ = $4^{\phantom{0}+\phantom{0}}$ = $4^{\phantom{0}}$ = \underline{\hspace{3cm}}
    \end{tabular}

    \vspace{1cm}

    \item \textbf{Potenzen mit gleicher Basis dividieren:}
    \textit{Regel:} $a^m : a^n = a^{m-n}$
    \vspace{0.5cm}

    \begin{tabular}{ll}
        a) $2^5 : 2^2$ = $2^{5-2}$ = $2^{\phantom{0}}$ = \underline{\hspace{3cm}} & b) $3^6 : 3^4$ = $3^{\phantom{0}-\phantom{0}}$ = $3^{\phantom{0}}$ = \underline{\hspace{3cm}} \\[3ex]
        c) $5^4 : 5^1$ = $5^{\phantom{0}-\phantom{0}}$ = $5^{\phantom{0}}$ = \underline{\hspace{3cm}} & d) $7^3 : 7^3$ = $7^{\phantom{0}-\phantom{0}}$ = $7^{\phantom{0}}$ = \underline{\hspace{3cm}}
    \end{tabular}

    \vspace{1cm}

    \item \textbf{Potenzen potenzieren:}
    \textit{Regel:} $(a^m)^n = a^{m \cdot n}$
    \vspace{0.5cm}

    \begin{enumerate}[label=\alph*)]
        \item $(2^2)^3$ = $2^{2 \cdot 3}$ = $2^{\phantom{0}}$ = \underline{\hspace{3cm}}
        \vspace{0.5cm}

        \item $(3^3)^2$ = $3^{\phantom{0} \cdot \phantom{0}}$ = $3^{\phantom{0}}$ = \underline{\hspace{3cm}}
        \vspace{0.5cm}

        \item $(5^1)^4$ = $5^{\phantom{0} \cdot \phantom{0}}$ = $5^{\phantom{0}}$ = \underline{\hspace{3cm}}
    \end{enumerate}

\end{enumerate}