\subsection*{Teil A: Terme vereinfachen (30 Minuten)}

\begin{enumerate}[label=\arabic*.]

    \item \textbf{Gleichartige Terme zusammenfassen:}
    \textit{Beispiel:} $3x + 5x = 8x$
    \vspace{0.5cm}

    \begin{tabular}{ll}
        a) $2x + 4x$ = \underline{\hspace{3cm}} & b) $7a - 3a$ = \underline{\hspace{3cm}} \\[3ex]
        c) $5y + 2y - y$ = \underline{\hspace{3cm}} & d) $8b - 5b + 2b$ = \underline{\hspace{3cm}} \\[3ex]
        e) $3x + 2y + 5x$ = \underline{\hspace{3cm}} & f) $4a - 2a + 3b$ = \underline{\hspace{3cm}}
    \end{tabular}

    \vspace{1cm}

    \item \textbf{Terme mit Potenzen zusammenfassen:}
    \textit{Beispiel:} $2x \cdot 3x = 6x^2$, $x^3 \cdot x^2 = x^5$
    \vspace{0.5cm}

    \begin{enumerate}[label=\alph*)]
        \item $x + 2x$ = \underline{\hspace{3cm}}
        \vspace{0.5cm}

        \item $3x \cdot 4x$ = $12x^{\phantom{0}}$ = \underline{\hspace{3cm}}
        \vspace{0.5cm}

        \item $x^2 \cdot x^3$ = $x^{\phantom{0}+\phantom{0}}$ = $x^{\phantom{0}}$ = \underline{\hspace{3cm}}
        \vspace{0.5cm}

        \item $5x^2 : 2x$ = $\dfrac{5x^2}{2x}$ = $\dfrac{5x^{\phantom{0}}}{2}$ = \underline{\hspace{3cm}}
        \vspace{0.5cm}

        \item $6x^4 : 3x^2$ = $\dfrac{6x^4}{3x^2}$ = $2x^{\phantom{0}}$ = \underline{\hspace{3cm}}
    \end{enumerate}

    \vspace{1cm}

    \item \textbf{Klammern aufl√∂sen:}
    \textit{Beispiel:} $3(x + 2) = 3x + 6$
    \vspace{0.5cm}

    \begin{enumerate}[label=\alph*)]
        \item $2(x + 3)$ = $2 \cdot x + 2 \cdot 3$ = \underline{\hspace{3cm}}
        \vspace{0.5cm}

        \item $4(a - 1)$ = $4 \cdot a - 4 \cdot 1$ = \underline{\hspace{3cm}}
        \vspace{0.5cm}

        \item $3(2x + 5)$ = $3 \cdot 2x + 3 \cdot 5$ = \underline{\hspace{3cm}}
        \vspace{0.5cm}

        \item $5(3y - 2)$ = $5 \cdot 3y - 5 \cdot 2$ = \underline{\hspace{3cm}}
    \end{enumerate}

\end{enumerate}